src/study/Nemonuri.Study.StratifiedNodes.Sample1/Adder.fst
@@ -28,15 +28,24 @@ let selector : (C.ancestor_list_given_selector nat nat) =
     N.get_value node
     )
 
-let aggregator : (Common.aggregator nat) =
+let aggregator_impl : (Common.aggregator nat) =
   fun v1 v2 -> (
     let msg = sprintf "%d + %d \n" v1 v2 in
     let _ = Log.debug_print_string msg in
     v1 + v2
   )
 
-let continue_predicate : (N.node nat -> nat -> bool) =
-  fun n t -> true
+let to_first_child_from_parent : (Common.aggregator nat) =
+  fun first_child_value parent_value -> (
+    let _ = Log.debug_print_string "to_first_child_from_parent: " in
+    aggregator_impl first_child_value parent_value
+  )
+
+let from_left_to_right : (Common.aggregator nat) =
+  fun first_child_value parent_value -> (
+    let _ = Log.debug_print_string "from_left_to_right: " in
+    aggregator_impl first_child_value parent_value
+  )
 
 let create_adder_node1 ()
   : Pure (node_t) True
@@ -62,7 +71,12 @@ let walk_adder_node (node:node_t)
   : Pure nat (requires is_adder_node node)
     (ensures fun _ -> true)
   =
-  W.walk node selector aggregator aggregator continue_predicate []
+  W.walk node selector 
+  to_first_child_from_parent 
+  from_left_to_right 
+  (Common.aggregated_identity nat) 
+  (C.always_continue_predicate nat nat)
+  []
 
 (*
 let _ = assert ( 
@@ -71,34 +85,63 @@ let _ = assert (
 )
 *)
 
+let forall_aggregator
+  : (Common.aggregator bool) =
+  fun v1 v2 -> (v1 && v2)
+
+let forall_continue_predicate (t:eqtype)
+  : (C.continue_predicate t bool) 
+  =
+  fun n v -> v
+
+let is_adder_node2 (node:node_t) (ancestors:C.next_head_given_ancestor_list node)
+  : Tot bool =
+  is_adder_node node
+
+let is_adder_node_really (node:node_t)
+  : Tot bool
+  = 
+  W.walk node is_adder_node2
+  forall_aggregator
+  forall_aggregator
+ (Common.aggregated_identity bool)
+ (forall_continue_predicate nat)
+ []
+
+(*
+let _ = assert ( is_adder_node_really (create_adder_node1 ()) )
+*)
 
 let main () = 
   let v1 = walk_adder_node (create_adder_node1 ()) in
   print_any v1;
   print_newline ();
   let v2 = walk_adder_node (create_adder_node2 ()) in
-  print_any v2
+  print_any v2; print_newline ();
+  print_any (is_adder_node_really (create_adder_node1 ())); print_newline ();
+  print_any (is_adder_node_really (create_adder_node2 ())); print_newline ()
 
 let _ = main ()
   
 (* 출력
 
-1 + 0
-1 + 2
-3 + 3
-3 + 3
-6 + 0
-4 + 0
-4 + 5
-6 + 9
+to_first_child_from_parent: 1 + 0 
+from_left_to_right: 1 + 2
+from_left_to_right: 3 + 3
+to_first_child_from_parent: 6 + 0
+to_first_child_from_parent: 4 + 0
+from_left_to_right: 4 + 5
+from_left_to_right: 6 + 9
 15
-4 + 0
-4 + 5
-9 + 0
-1 + 0
-1 + 2
-3 + 3
-9 + 6
+to_first_child_from_parent: 4 + 0
+from_left_to_right: 4 + 5
+to_first_child_from_parent: 9 + 0
+to_first_child_from_parent: 1 + 0
+from_left_to_right: 1 + 2
+from_left_to_right: 3 + 3
+from_left_to_right: 9 + 6
 15
+true
+true
 
 *)
