src/study/Nemonuri.Study.CSharpSyntaxRewriter2.Modifier2/Nemonuri.StratifiedNodes.Children.Types.fst
@@ -1,0 +1,8 @@
+module Nemonuri.StratifiedNodes.Children.Types
+
+module N = Nemonuri.StratifiedNodes.Nodes
+
+//--- type defenitions ---
+let continue_predicate (t:eqtype) (t2:Type)
+  = N.node t -> t2 -> Tot bool
+//---|
