src/study/Nemonuri.Study.CSharpSyntaxRewriter2.Modifier2/Nemonuri.StratifiedNodes.Common.fst
@@ -4,6 +4,10 @@ module L = FStar.List.Tot
 
 //--- type definitions ---
 let aggregator (t:Type) = (aggregated:t) -> (aggregating:t) -> t
+
+let aggregated_identity (t:Type) 
+  : (aggregator t) =
+  fun aggregated aggregating -> aggregated
 //---|
 
 //--- propositions ---
