src/study/Nemonuri.Study.CSharpSyntaxRewriter2.Modifier2/Nemonuri.StratifiedNodes.Walkers.fst
@@ -13,9 +13,10 @@ module Common = Nemonuri.StratifiedNodes.Common
 let rec walk #t #t2
   (node:N.node t)
   (selector:C.ancestor_list_given_selector t t2)
-  (child_parent_aggregator:Common.aggregator t2) 
-  (left_right_aggregator:Common.aggregator t2)
-  (continue_predicate:N.node t -> t2 -> bool)
+  (to_first_child_from_parent:Common.aggregator t2) 
+  (from_left_to_right:Common.aggregator t2)
+  (from_last_child_to_parent:Common.aggregator t2) 
+  (continue_predicate:C.continue_predicate t t2)
   (ancestors:C.next_head_given_ancestor_list node)
   : Tot t2 (decreases (node.level)) =
   let v1 = selector node ancestors in
@@ -24,7 +25,16 @@ let rec walk #t #t2
   else
     let next_ancestors = C.concatenate_as_ancestor_list node ancestors in
     C.select_and_aggregate_from_children
-      node (fun child ancestors -> 
-        (walk child selector child_parent_aggregator left_right_aggregator continue_predicate ancestors)
-      ) child_parent_aggregator left_right_aggregator continue_predicate next_ancestors v1
+      node v1
+      (fun child ancestors -> (
+        walk child selector 
+        to_first_child_from_parent 
+        from_left_to_right 
+        from_last_child_to_parent
+        continue_predicate ancestors)
+      ) 
+      to_first_child_from_parent 
+      from_left_to_right 
+      from_last_child_to_parent
+      continue_predicate next_ancestors
 //---|
